src/HOL/Word/Conversions.thy
@@ -13,7 +13,8 @@ begin
 
 hide_const (open) unat uint sint word_of_int ucast scast
 
-subsection \<open>Conversions to words\<close>
+
+subsection \<open>Conversions to word\<close>
 
 abbreviation word_of_nat :: \<open>nat \<Rightarrow> 'a::len word\<close>
   where \<open>word_of_nat \<equiv> of_nat\<close>
@@ -57,81 +58,10 @@ lemma word_of_int_eq_0_iff [simp]:
   \<open>word_of_int k = (0 :: 'a::len word) \<longleftrightarrow> 2 ^ LENGTH('a) dvd k\<close>
   using of_int_word_eq_iff [where ?'a = 'a, of k 0] by (simp add: take_bit_eq_0_iff)
 
-lemma int_AND_eq:
-  \<open>int (m AND n) = int m AND int n\<close>
-  by (rule bit_eqI) (simp add: bit_and_iff)
 
-lemma int_OR_eq:
-  \<open>int (m OR n) = int m OR int n\<close>
-  by (rule bit_eqI) (simp add: bit_or_iff)
+subsection \<open>Conversion from word\<close>
 
-lemma int_XOR_eq:
-  \<open>int (m XOR n) = int m XOR int n\<close>
-  by (rule bit_eqI) (simp add: bit_xor_iff)
-
-context semiring_bit_operations
-begin
-
-lemma push_bit_and [simp]:
-  \<open>push_bit n (a AND b) = push_bit n a AND push_bit n b\<close>
-  by (rule bit_eqI) (auto simp add: bit_push_bit_iff bit_and_iff)
-
-lemma push_bit_or [simp]:
-  \<open>push_bit n (a OR b) = push_bit n a OR push_bit n b\<close>
-  by (rule bit_eqI) (auto simp add: bit_push_bit_iff bit_or_iff)
-
-lemma push_bit_xor [simp]:
-  \<open>push_bit n (a XOR b) = push_bit n a XOR push_bit n b\<close>
-  by (rule bit_eqI) (auto simp add: bit_push_bit_iff bit_xor_iff)
-
-lemma drop_bit_and [simp]:
-  \<open>drop_bit n (a AND b) = drop_bit n a AND drop_bit n b\<close>
-  by (rule bit_eqI) (auto simp add: bit_drop_bit_eq bit_and_iff)
-
-lemma drop_bit_or [simp]:
-  \<open>drop_bit n (a OR b) = drop_bit n a OR drop_bit n b\<close>
-  by (rule bit_eqI) (auto simp add: bit_drop_bit_eq bit_or_iff)
-
-lemma drop_bit_xor [simp]:
-  \<open>drop_bit n (a XOR b) = drop_bit n a XOR drop_bit n b\<close>
-  by (rule bit_eqI) (auto simp add: bit_drop_bit_eq bit_xor_iff)
-
-end
-
-lemma bit_word_of_nat_iff:
-  \<open>bit (word_of_nat m :: 'a::len word) n \<longleftrightarrow> n < LENGTH('a) \<and> bit m n\<close>
-  by transfer simp
-
-lemma bit_word_of_int_iff:
-  \<open>bit (word_of_int k :: 'a::len word) n \<longleftrightarrow> n < LENGTH('a) \<and> bit k n\<close>
-  by transfer simp
-
-lemma word_of_nat_AND_eq:
-  \<open>word_of_nat (m AND n) = word_of_nat m AND word_of_nat n\<close>
-  by (rule bit_eqI) (auto simp add: bit_word_of_nat_iff bit_and_iff)
-
-lemma word_of_int_AND_eq:
-  \<open>word_of_int (k AND l) = word_of_int k AND word_of_int l\<close>
-  by (rule bit_eqI) (auto simp add: bit_word_of_int_iff bit_and_iff)
-
-lemma word_of_nat_OR_eq:
-  \<open>word_of_nat (m OR n) = word_of_nat m OR word_of_nat n\<close>
-  by (rule bit_eqI) (auto simp add: bit_word_of_nat_iff bit_or_iff)
-
-lemma word_of_int_OR_eq:
-  \<open>word_of_int (k OR l) = word_of_int k OR word_of_int l\<close>
-  by (rule bit_eqI) (auto simp add: bit_word_of_int_iff bit_or_iff)
-
-lemma word_of_nat_XOR_eq:
-  \<open>word_of_nat (m XOR n) = word_of_nat m XOR word_of_nat n\<close>
-  by (rule bit_eqI) (auto simp add: bit_word_of_nat_iff bit_xor_iff)
-
-lemma word_of_int_XOR_eq:
-  \<open>word_of_int (k XOR l) = word_of_int k XOR word_of_int l\<close>
-  by (rule bit_eqI) (auto simp add: bit_word_of_int_iff bit_xor_iff)
-
-
-subsection \<open>Conversion from words\<close>
+subsubsection \<open>Generic unsigned conversion\<close>
 
 context semiring_1
 begin
@@ -162,6 +92,114 @@ lemma word_eq_iff_unsigned:
   by (auto intro: unsigned_word_eqI)
 
 end
+
+context semiring_bits
+begin
+
+lemma bit_unsigned_iff:
+  \<open>bit (unsigned w) n \<longleftrightarrow> 2 ^ n \<noteq> 0 \<and> bit w n\<close>
+  for w :: \<open>'b::len word\<close>
+  by (transfer fixing: bit) (simp add: bit_of_nat_iff bit_nat_iff bit_take_bit_iff)
+
+end
+
+context semiring_bit_shifts
+begin
+
+lemma unsigned_push_bit_eq:
+  \<open>unsigned (push_bit n w) = take_bit LENGTH('b) (push_bit n (unsigned w))\<close>
+  for w :: \<open>'b::len word\<close>
+proof (rule bit_eqI)
+  fix m
+  assume \<open>2 ^ m \<noteq> 0\<close>
+  show \<open>bit (unsigned (push_bit n w)) m = bit (take_bit LENGTH('b) (push_bit n (unsigned w))) m\<close>
+  proof (cases \<open>n \<le> m\<close>)
+    case True
+    with \<open>2 ^ m \<noteq> 0\<close> have \<open>2 ^ (m - n) \<noteq> 0\<close>
+      by (metis (full_types) diff_add exp_add_not_zero_imp)
+    with True show ?thesis
+      by (simp add: bit_unsigned_iff bit_push_bit_iff Parity.bit_push_bit_iff bit_take_bit_iff ac_simps exp_eq_zero_iff not_le)
+  next
+    case False
+    then show ?thesis
+      by (simp add: not_le bit_unsigned_iff bit_push_bit_iff Parity.bit_push_bit_iff bit_take_bit_iff)
+  qed
+qed
+
+lemma unsigned_take_bit_eq:
+  \<open>unsigned (take_bit n w) = take_bit n (unsigned w)\<close>
+  for w :: \<open>'b::len word\<close>
+  by (rule bit_eqI) (simp add: bit_unsigned_iff bit_take_bit_iff Parity.bit_take_bit_iff)
+
+end
+
+context semiring_bit_operations
+begin
+
+lemma unsigned_and_eq:
+  \<open>unsigned (v AND w) = unsigned v AND unsigned w\<close>
+  for v w :: \<open>'b::len word\<close>
+  by (rule bit_eqI) (simp add: bit_unsigned_iff bit_and_iff Bit_Operations.bit_and_iff)
+
+lemma unsigned_or_eq:
+  \<open>unsigned (v OR w) = unsigned v OR unsigned w\<close>
+  for v w :: \<open>'b::len word\<close>
+  by (rule bit_eqI) (simp add: bit_unsigned_iff bit_or_iff Bit_Operations.bit_or_iff)
+
+lemma unsigned_xor_eq:
+  \<open>unsigned (v XOR w) = unsigned v XOR unsigned w\<close>
+  for v w :: \<open>'b::len word\<close>
+  by (rule bit_eqI) (simp add: bit_unsigned_iff bit_xor_iff Bit_Operations.bit_xor_iff)
+
+end
+
+context ring_bit_operations
+begin
+
+lemma unsigned_not_eq:
+  \<open>unsigned (NOT w) = take_bit LENGTH('b) (NOT (unsigned w))\<close>
+  for w :: \<open>'b::len word\<close>
+  by (rule bit_eqI)
+    (simp add: bit_unsigned_iff bit_take_bit_iff bit_not_iff Bit_Operations.bit_not_iff exp_eq_zero_iff not_le)
+
+end
+
+lemma unsigned_of_nat [simp]:
+  \<open>unsigned (word_of_nat n :: 'a::len word) = of_nat (take_bit LENGTH('a) n)\<close>
+  by transfer (simp add: nat_eq_iff take_bit_of_nat)
+
+lemma unsigned_of_int [simp]:
+  \<open>unsigned (word_of_int n :: 'a::len word) = of_int (take_bit LENGTH('a) n)\<close>
+  by transfer (simp add: nat_eq_iff take_bit_of_nat)
+
+context unique_euclidean_semiring_numeral
+begin
+
+lemma unsigned_greater_eq:
+  \<open>0 \<le> unsigned w\<close> for w :: \<open>'b::len word\<close>
+  by (transfer fixing: less_eq) simp
+
+lemma unsigned_less:
+  \<open>unsigned w < 2 ^ LENGTH('b)\<close> for w :: \<open>'b::len word\<close>
+  by (transfer fixing: less) (simp add: take_bit_int_less_exp)
+
+end
+
+context linordered_semidom
+begin
+
+lemma word_less_eq_iff_unsigned:
+  "a \<le> b \<longleftrightarrow> unsigned a \<le> unsigned b"
+  by (transfer fixing: less_eq) (simp add: nat_le_eq_zle)
+
+lemma word_less_iff_unsigned:
+  "a < b \<longleftrightarrow> unsigned a < unsigned b"
+  by (transfer fixing: less) (auto dest: preorder_class.le_less_trans [OF take_bit_nonnegative])
+
+end
+
+
+subsubsection \<open>Generic signed conversion\<close>
 
 context ring_1
 begin
@@ -197,6 +235,99 @@ lemma word_eq_iff_signed:
   by (auto intro: signed_word_eqI)
 
 end
+
+context ring_bit_operations
+begin
+
+lemma bit_signed_iff:
+  \<open>bit (signed w) n \<longleftrightarrow> 2 ^ n \<noteq> 0 \<and> bit w (min (LENGTH('b) - Suc 0) n)\<close>
+  for w :: \<open>'b::len word\<close>
+  by (transfer fixing: bit) (auto simp add: bit_of_int_iff bit_signed_take_bit_iff min_def)
+
+lemma signed_push_bit_eq:
+  \<open>signed (push_bit n w) = take_bit (LENGTH('b) - Suc 0) (push_bit n (signed w))
+    OR of_bool (n < LENGTH('b) \<and> bit w (LENGTH('b) - Suc n)) * NOT (mask (LENGTH('b) - Suc 0))\<close>
+  for w :: \<open>'b::len word\<close>
+proof (rule bit_eqI)
+  fix m
+  assume \<open>2 ^ m \<noteq> 0\<close>
+  define q where \<open>q = LENGTH('b) - Suc 0\<close>
+  then have *: \<open>LENGTH('b) = Suc q\<close>
+    by simp
+  show \<open>bit (signed (push_bit n w)) m \<longleftrightarrow>
+    bit (take_bit (LENGTH('b) - Suc 0) (push_bit n (signed w)) OR
+      of_bool (n < LENGTH('b) \<and> bit w (LENGTH('b) - Suc n)) * NOT (mask (LENGTH('b) - Suc 0))) m\<close>
+  proof (cases \<open>n \<le> m\<close>)
+    case True
+    with \<open>2 ^ m \<noteq> 0\<close> have \<open>2 ^ (m - n) \<noteq> 0\<close>
+      by (metis (full_types) diff_add exp_add_not_zero_imp)
+    with True show ?thesis
+      by (auto simp add: * bit_signed_iff bit_push_bit_iff Parity.bit_push_bit_iff bit_or_iff bit_take_bit_iff bit_not_iff bit_mask_iff exp_eq_zero_iff min_def)
+  next
+    case False
+    then show ?thesis
+      by (simp add: * bit_signed_iff bit_push_bit_iff Parity.bit_push_bit_iff bit_or_iff bit_take_bit_iff bit_not_iff bit_mask_iff)
+  qed
+qed
+
+lemma signed_take_bit_eq:
+  \<open>signed (take_bit n w) = (if n < LENGTH('b) then take_bit n (signed w) else signed w)\<close>
+  for w :: \<open>'b::len word\<close>
+  by (transfer fixing: take_bit; cases \<open>LENGTH('b)\<close>)
+    (auto simp add: signed_take_bit_take_bit take_bit_signed_take_bit take_bit_of_int min_def)
+
+lemma signed_not_eq:
+  \<open>signed (NOT w) = take_bit LENGTH('b) (NOT (signed w)) OR of_bool (bit (NOT (signed w)) LENGTH('b)) * NOT (mask LENGTH('b))\<close>
+  for w :: \<open>'b::len word\<close>
+proof (rule bit_eqI)
+  fix n
+  assume \<open>2 ^ n \<noteq> 0\<close>
+  show \<open>bit (signed (NOT w)) n \<longleftrightarrow>
+    bit (take_bit LENGTH('b) (NOT (signed w)) OR
+    of_bool (bit (NOT (signed w)) LENGTH('b)) * NOT (mask LENGTH('b))) n\<close>
+  proof (cases \<open>LENGTH('b) \<le> n\<close>)
+    case False
+    then show ?thesis
+      by (auto simp add: bit_signed_iff bit_not_iff bit_or_iff bit_take_bit_iff bit_mask_iff Bit_Operations.bit_not_iff exp_eq_zero_iff)
+  next
+    case True
+    moreover define q where \<open>q = n - LENGTH('b)\<close>
+    ultimately have \<open>n = LENGTH('b) + q\<close>
+      by simp
+    with \<open>2 ^ n \<noteq> 0\<close> have \<open>2 ^ q \<noteq> 0\<close> \<open>2 ^ LENGTH('b) \<noteq> 0\<close>
+      by (simp_all add: power_add) (use mult_not_zero in blast)+
+    then show ?thesis
+      by (simp add: bit_signed_iff bit_not_iff bit_or_iff bit_take_bit_iff bit_mask_iff Bit_Operations.bit_not_iff exp_eq_zero_iff min_def not_le not_less le_diff_conv le_Suc_eq)
+  qed
+qed
+
+lemma signed_and_eq:
+  \<open>signed (v AND w) = signed v AND signed w\<close>
+  for v w :: \<open>'b::len word\<close>
+  by (rule bit_eqI) (simp add: bit_signed_iff bit_and_iff Bit_Operations.bit_and_iff)
+
+lemma signed_or_eq:
+  \<open>signed (v OR w) = signed v OR signed w\<close>
+  for v w :: \<open>'b::len word\<close>
+  by (rule bit_eqI) (simp add: bit_signed_iff bit_or_iff Bit_Operations.bit_or_iff)
+
+lemma signed_xor_eq:
+  \<open>signed (v XOR w) = signed v XOR signed w\<close>
+  for v w :: \<open>'b::len word\<close>
+  by (rule bit_eqI) (simp add: bit_signed_iff bit_xor_iff Bit_Operations.bit_xor_iff)
+
+end
+
+lemma signed_of_nat [simp]:
+  \<open>signed (word_of_nat n :: 'a::len word) = of_int (signed_take_bit (LENGTH('a) - Suc 0) (int n))\<close>
+  by transfer simp
+
+lemma signed_of_int [simp]:
+  \<open>signed (word_of_int n :: 'a::len word) = of_int (signed_take_bit (LENGTH('a) - Suc 0) n)\<close>
+  by transfer simp
+
+
+subsubsection \<open>Important special cases\<close>
 
 abbreviation unat :: \<open>'a::len word \<Rightarrow> nat\<close>
   where \<open>unat \<equiv> unsigned\<close>
@@ -257,10 +388,6 @@ qed
 
 end
 
-lemma unsigned_of_nat [simp]:
-  \<open>unsigned (of_nat n :: 'a::len word) = of_nat (take_bit LENGTH('a) n)\<close>
-  by transfer (simp add: nat_eq_iff take_bit_of_nat)
-
 lemma of_nat_unat [simp]:
   \<open>of_nat (unat w) = unsigned w\<close>
   by transfer simp
@@ -269,39 +396,65 @@ lemma of_int_uint [simp]:
   \<open>of_int (uint w) = unsigned w\<close>
   by transfer simp
 
-context unique_euclidean_semiring_numeral
-begin
+lemma unat_div_distrib:
+  \<open>unat (v div w) = unat v div unat w\<close>
+proof transfer
+  fix k l
+  have \<open>nat (take_bit LENGTH('a) k) div nat (take_bit LENGTH('a) l) \<le> nat (take_bit LENGTH('a) k)\<close>
+    by (rule div_le_dividend)
+  also have \<open>nat (take_bit LENGTH('a) k) < 2 ^ LENGTH('a)\<close>
+    by (simp add: nat_less_iff take_bit_int_less_exp)
+  finally show \<open>(nat \<circ> take_bit LENGTH('a)) (take_bit LENGTH('a) k div take_bit LENGTH('a) l) =
+    (nat \<circ> take_bit LENGTH('a)) k div (nat \<circ> take_bit LENGTH('a)) l\<close>
+    by (simp add: nat_take_bit_eq div_int_pos_iff nat_div_distrib take_bit_eq_self)
+qed
 
-lemma unsigned_greater_eq:
-  \<open>0 \<le> unsigned w\<close> for w :: \<open>'b::len word\<close>
-  by (transfer fixing: less_eq) simp
+lemma unat_mod_distrib:
+  \<open>unat (v mod w) = unat v mod unat w\<close>
+proof transfer
+  fix k l
+  have \<open>nat (take_bit LENGTH('a) k) mod nat (take_bit LENGTH('a) l) \<le> nat (take_bit LENGTH('a) k)\<close>
+    by (rule mod_less_eq_dividend)
+  also have \<open>nat (take_bit LENGTH('a) k) < 2 ^ LENGTH('a)\<close>
+    by (simp add: nat_less_iff take_bit_int_less_exp)
+  finally show \<open>(nat \<circ> take_bit LENGTH('a)) (take_bit LENGTH('a) k mod take_bit LENGTH('a) l) =
+    (nat \<circ> take_bit LENGTH('a)) k mod (nat \<circ> take_bit LENGTH('a)) l\<close>
+    by (simp add: nat_take_bit_eq mod_int_pos_iff less_le nat_mod_distrib take_bit_eq_self)
+qed
 
-lemma unsigned_less:
-  \<open>unsigned w < 2 ^ LENGTH('b)\<close> for w :: \<open>'b::len word\<close>
-  by (transfer fixing: less) (simp add: take_bit_int_less_exp)
+lemma uint_div_distrib:
+  \<open>uint (v div w) = uint v div uint w\<close>
+proof -
+  have \<open>int (unat (v div w)) = int (unat v div unat w)\<close>
+    by (simp add: unat_div_distrib)
+  then show ?thesis
+    by (simp add: of_nat_div)
+qed
 
-end
-
-context linordered_semidom
-begin
-
-lemma word_less_eq_iff_unsigned:
-  "a \<le> b \<longleftrightarrow> unsigned a \<le> unsigned b"
-  by (transfer fixing: less_eq) (simp add: nat_le_eq_zle)
-
-lemma word_less_iff_unsigned:
-  "a < b \<longleftrightarrow> unsigned a < unsigned b"
-  by (transfer fixing: less) (auto dest: preorder_class.le_less_trans [OF take_bit_nonnegative])
-
-end
-
-lemma signed_of_int [simp]:
-  \<open>signed (word_of_int k :: 'a::len word) = of_int (signed_take_bit (LENGTH('a) - 1) k)\<close>
-  by transfer simp
+lemma uint_mod_distrib:
+  \<open>uint (v mod w) = uint v mod uint w\<close>
+proof -
+  have \<open>int (unat (v mod w)) = int (unat v mod unat w)\<close>
+    by (simp add: unat_mod_distrib)
+  then show ?thesis
+    by (simp add: of_nat_mod)
+qed
 
 lemma of_int_sint [simp]:
   \<open>of_int (sint a) = signed a\<close>
   by transfer (simp_all add: take_bit_signed_take_bit)
+
+lemma sint_not_eq:
+  \<open>sint (NOT w) = signed_take_bit LENGTH('a) (NOT (sint w))\<close>
+  for w :: \<open>'a::len word\<close>
+  by (simp add: signed_not_eq signed_take_bit_unfold)
+
+lemma sint_push_bit_eq:
+  \<open>signed (push_bit n w) = signed_take_bit (LENGTH('a) - 1) (push_bit n (signed w))\<close>
+  for w :: \<open>'a::len word\<close>
+  by (transfer fixing: n; cases \<open>LENGTH('a)\<close>)
+     (auto simp add: signed_take_bit_def bit_concat_bit_iff bit_push_bit_iff bit_take_bit_iff bit_or_iff le_diff_conv2,
+        auto simp add: take_bit_push_bit not_less concat_bit_eq_iff take_bit_concat_bit_eq le_diff_conv2)
 
 lemma sint_greater_eq:
   \<open>- (2 ^ (LENGTH('a) - 1)) \<le> sint w\<close> for w :: \<open>'a::len word\<close>
@@ -320,6 +473,6 @@ qed
 lemma sint_less:
   \<open>sint w < 2 ^ (LENGTH('a) - 1)\<close> for w :: \<open>'a::len word\<close>
   by (cases \<open>bit w (LENGTH('a) - 1)\<close>; transfer)
-    (simp_all add: signed_take_bit_eq signed_take_bit_eq_or take_bit_int_less_exp not_eq_complement mask_eq_exp_minus_1 OR_upper)
+    (simp_all add: signed_take_bit_eq signed_take_bit_unfold take_bit_int_less_exp not_eq_complement mask_eq_exp_minus_1 OR_upper)
 
 end
